tests/coq/hashmap/Notes.v
@@ -1,19 +1,13 @@
 
-Require Import Primitives.
-Import Primitives.
+Require Import Primitives_Ext.
 Require Import Coq.ZArith.ZArith.
-Require Import Coq.Lists.List.
-Local Open Scope Primitives_scope.
-Require Import Hashmap_Types.
-Import Hashmap_Types.
-Require Import Hashmap_Funs.
-Import Hashmap_Funs.
 Require Import Lia.
-Require Import Coq.Unicode.Utf8.
-Require Import Coq.Program.Basics.
-Require Import Coq.Program.Equality.
-Require Import Coq.Logic.ProofIrrelevance.
-Require Import Coq.Bool.Bool.
+
+(* SSReflect settings *)
+From Coq Require Import ssreflect ssrfun ssrbool.
+Set Implicit Arguments.
+Unset Strict Implicit.
+Unset Printing Implicit Defensive.
 
 (*    +----------------+
       | Hint databases |
@@ -119,11 +113,153 @@ Search (S _ >= _).
 (*
     On Ltac:
 
-  How to visit a lambda-term (recursively inspect abstractions, applications and variables) ?
-
   How to match a fixpoint ?
 
   How to do a breath-first search ?
 *)
 
+(*    +-----------+
+      | SSReflect |
+      +-----------+
+*)
+(*
+A new set of tactics and tacticals for Coq :
+The reflection is for being able to easily switch between Prop and Bool.
+It is small-scale because it's applied locally (not full reflection by default).
+For that, some patterns are adopted eg. CoInductive props (see https://hal.inria.fr/inria-00407778/document).
+The tactics act on the top of the goal (or 'proof stack').
+That allows to not duplicate them for goal or hypothesis, e.g. :
+"move=> x" = "intro x", "move: x" = "revert x".
+Also lots of small shortcut, e.g. on rewrite :
+ - "rewrite {} f" = "rewrite f; clear f"
+ - "rewrite /f" = "unfold f"
+ - "rewrite -[n.+1 + m]/(n + m).+1" ~= "change ((S n) + m) with (S (n + m))" (patterns for rewrite !)
+Encourages some practices such as finishing (sub-)goals with "by ..." tactical for early error.
+SSReflect also block "simpl" on several functions (e.g. addition in nat or Z).
+However, it aims to compute better than by default :
+e.g. on nat, "n <= m -> 51 + n <= 51 + m" is proven by computation (but is usually stuck).
+*)
 
+(*    +---------+
+      | Lithium |
+      +---------+
+*)
+(*
+This is the REfinedC engine to automatize proofs on a deep embedding of C in Coq. The goal here is to understand its top-level tactic "liStep" which advances on the goal (we want something similar), especially how it relates to typeclass inference.
+As in Iris & std++, the simplification on Z is disabled. We may want something similar on scalars & vectors to avoid expanding existentials, provided we have a specialized tactic to reduce constants (to_Z 1%usize ~> 1).
+The "xxx_hook" ltac functions can be replaced with debug variants to print a trace.
+It's a big engine which rebuilds most notions. Reduction comes from Iris's reduction.pm_eval.
+The std++ file "base.v" is very instructive. In particular, it tells us that
+- Usual "refine" uses are separated from the typeclass "refine", by using "notypeclasses refine" resp. "tc_solve" (which acts like "apply _" but only for typeclasses).
+- The typeclasses such as "TCOr" copy the "or" connective. They are used when we want to leverage the typeclass search.
+*)
+(*
+Mentions:
+RefinedC does NOT mention "tc_solve/opaque", "SimplifyHyp/Goal", almost no "TCXXX" (one "TCForall2").
+*)
+
+(* Avoid the backtracking behavior of "typeclasses eauto", however typeclasses are usually resolved with comon tactics e.g. "exact _". *)
+Ltac tc_solve :=
+  solve [once (typeclasses eauto)].
+
+(* Taken from "stdpp/base.v" *)
+
+Inductive TCOr (P1 P2 : Prop) : Prop :=
+  | TCOr_l: P1 -> TCOr P1 P2
+  | TCOr_r: P2 -> TCOr P1 P2.
+Existing Class TCOr.
+Global Existing Instance TCOr_l | 9.
+Global Existing Instance TCOr_r | 10.
+Global Hint Mode TCOr ! ! : typeclass_instances.
+
+Inductive TCAnd (P1 P2 : Prop) : Prop := TCAnd_intro : P1 -> P2 -> TCAnd P1 P2.
+Existing Class TCAnd.
+Global Existing Instance TCAnd_intro.
+Global Hint Mode TCAnd ! ! : typeclass_instances.
+
+Inductive TCTrue : Prop := TCTrue_intro : TCTrue.
+Existing Class TCTrue.
+Global Existing Instance TCTrue_intro.
+
+Inductive TCEq {A} (x : A) : A -> Prop := TCEq_refl : TCEq x x.
+Existing Class TCEq.
+Global Existing Instance TCEq_refl.
+Global Hint Mode TCEq ! - - : typeclass_instances.
+
+Lemma tc_eq_refl {A} (x1 x2 : A) : TCEq x1 x2 <-> x1 = x2.
+Proof. split; now destruct 1. Qed.
+
+(* From "Lithium/simpl_instances.v" *)
+Class SimplImpl (P : Prop) (Ps : Prop -> Prop) :=
+  simpl_impl T: (Ps T) <-> (P -> T).
+  
+Global Instance simpl_and_impl (P1 P2 : Prop):
+  SimplImpl (P1 /\ P2) (fun T => P1 -> P2 -> T).
+Proof. split; intuition. Qed.
+
+(* Tests *)
+
+(* Issues:
+- cannot precise lookup (any x:T)
+- no information if the term is opaque
+*)
+Class SpecMap {T} (x: T) := {
+  spec_lem : Prop;
+  spec_val : spec_lem;
+}.
+
+Lemma nat_sub_add (a b: nat) : a >= b -> (a - b) + b = a.
+Proof. lia. Qed.
+
+Global Instance spec_nat_sub : SpecMap Nat.sub :=
+  {| spec_lem := _;
+     spec_val := nat_sub_add;
+  |}.
+  
+Definition egg : SpecMap Nat.sub (* := ltac:(tc_solve)*) .
+Proof.
+pose (L := (ltac:(tc_solve): SpecMap Nat.sub)).
+simpl in L.
+exact L.
+Defined.
+
+Lemma nat_double_sub (a: nat) :
+  (a - a) + a = a.
+Proof.
+(* Ideally, we get the instance for the good lemma and apply it. *)
+set (L:= (ltac:(tc_solve): SpecMap Nat.sub)).
+simpl in L.
+assert (S := spec_val a a).
+simpl in S.
+Abort.
+
+Lemma tc_or_refl {A B: Prop} : TCOr A B -> A \/ B.
+Proof. intuition. Qed.
+Lemma tc_and_refl {A B: Prop} : TCAnd A B -> A /\ B.
+Proof. intuition. Qed.
+
+Example tc_or_left_fail {A B: Prop} : A -> A \/ B.
+Proof. Fail exact _. Abort.
+
+Example tc_or_left {A B: Prop} : A -> A \/ B.
+Proof. intro. apply tc_or_refl. revert H. exact _. Qed.
+
+(*    +--------+
+      | aeStep |
+      +--------+
+*)
+(*
+We want a high-level action which simplifies the goal w.r.t. data specific to Aeneas, which fetches and progress on the head variable (no "context [...]" query !).
+Ideally, we would only need to add the needed lemmas for "lia" in the context and run "aeStep" until the next step is not specific to Aeneas.
+Because we cannot seem to match "fix" in ltac, we can still aim to unfold/refold and match the fuel pattern.
+We should avoid to "simpl" to even block it on Aeneas values (to avoid existential variables expansion), but manage to always simplify constants (e.g. "to_Z 2%usize", also perhaps "to_list [vec of known elements]").
+*)
+
+(*
+Typeclass v2
+
+Idea: typeclass as map between term (e.g. u32_add) and lemma to apply.
+It allows us to avoid referring to the lemma of a function, only to the function itself.
+
+Issues: does not help to see which functions are supported. For automation, we need to unfold the lemma obtained explicitely.
+*)
