tests/coq/hashmap/Primitives_Ext.v
@@ -1,6 +1,6 @@
 
 (* TODO: Cleanup imports and scopes *)
-Require Import Primitives.
+Require Export Primitives.
 Import Primitives.
 Require Import Coq.ZArith.ZArith.
 Local Open Scope Primitives_scope.
@@ -23,6 +23,9 @@ Require ltac2_ident_to_string.
 
 Module Primitives_Ext.
 
+(* Improves "rewrite", which was before missing some terms without any good reason. *)
+Set Keyed Unification.
+
 Ltac string_to_ident s := ltac2_string_to_ident.string_to_ident s.
 
 Notation ident_to_string id :=
@@ -33,25 +36,26 @@ Notation ident_to_string id :=
     +------------------------------+
 *)
 
-Lemma neg_impl {A B: Prop} : (A -> B) -> ~B -> ~A.
+Lemma neg_impl {A B: Prop} : (A → B) → ~B → ~A.
 intuition. Qed.
 
-Lemma neg_equiv {A B: Prop} : A <-> B -> ~A <-> ~B.
+Lemma neg_equiv {A B: Prop} : A ↔ B → ~A ↔ ~B.
 apply not_iff_compat. Qed.
 
-Lemma orb_dis {A B: bool} : (A || B) = false <-> A = false /\ B = false.
+Lemma orb_dis {A B: bool} : (A || B) = false ↔ A = false ∧ B = false.
 destruct A, B ; intuition. Qed.
 
-Lemma Ztrans_le_lt a b c : a < b -> b <= c -> a <= c.
+(* TODO: Is there a "≤" notation for "Z" (or only "Nat") ? *)
+Lemma Ztrans_le_lt a b c : a < b → b <= c → a <= c.
 intuition. Qed.
 
-Lemma Zsucc_le_mono n m : n <= m -> n <= Z.succ m.
+Lemma Zsucc_le_mono n m : n <= m → n <= Z.succ m.
 intuition. Qed.
 
-Lemma Zpred_le_mono n m : n <= m -> Z.pred n <= m.
+Lemma Zpred_le_mono n m : n <= m → Z.pred n <= m.
 intuition. Qed.
 
-Lemma Zle_antisym {n m} : (n <= m) <-> (m >= n).
+Lemma Zle_antisym {n m} : (n <= m) ↔ (m >= n).
 intuition. Qed.
 
 Lemma Zeqb_sym {n m} : (n =? m) = (m =? n).
@@ -76,7 +80,7 @@ Definition res_of_opt {T} (o: option T) : result T :=
     | None   => Fail_ Failure
     end.
 
-Definition res_fmap {A B} (x: result A) (f: A -> B) : result B :=
+Definition res_fmap {A B} (x: result A) (f: A → B) : result B :=
     x' <- x; Return (f x').
 
 Lemma res_bind_id {T} {x: result T} : (v <- x; Return v) = x.
@@ -85,7 +89,7 @@ now destruct x ; simpl.
 Qed.
 
 (* Useful to simplify trivial bindings without mentioning f *)
-Lemma res_bind_value {A B} {f: A -> result B} (x: A) :
+Lemma res_bind_value {A B} {f: A → result B} (x: A) :
     (v <- Return x ; f v) = f x.
 Proof.
 trivial.
@@ -97,7 +101,7 @@ Qed.
 *)
 
 (* Uses proof irrelevance so vector underlying lists can be equated *)
-Lemma vec_list_inj {T} {a b: vec T} : (vec_to_list a = vec_to_list b) -> (a = b).
+Lemma vec_list_inj {T} {a b: vec T} : (vec_to_list a = vec_to_list b) → (a = b).
 Proof.
 destruct a, b.
 apply ProofIrrelevanceTheory.subset_eq_compat.
@@ -183,14 +187,14 @@ Definition scalar_ty_of {ty} (n: scalar ty) := ty.
 Hint Unfold usize_to_nat : core.
 
 (* Uses proof irrelevance so scalars with the same number can be equated *)
-Lemma scalar_Z_inj {ty} {n m: scalar ty} : (to_Z n = to_Z m) -> (n = m).
+Lemma scalar_Z_inj {ty} {n m: scalar ty} : (to_Z n = to_Z m) → (n = m).
 Proof.
 destruct m, n.
 apply ProofIrrelevanceTheory.subset_eq_compat.
 Qed.
 
 (* Usize lemmas can be generalized for positive scalars *)
-Lemma usize_nat_inj {n m: usize} : (usize_to_nat n = usize_to_nat m) <-> (n = m).
+Lemma usize_nat_inj {n m: usize} : (usize_to_nat n = usize_to_nat m) ↔ (n = m).
 Proof.
 split ; intro H.
 - unfold usize_to_nat in H.
@@ -203,7 +207,7 @@ Qed.
 
 (* It's a simple implication in "scalar_in_bounds_valid" *)
 Lemma scalar_in_bounds_valid2 (ty: scalar_ty) (x: Z) :
-  scalar_in_bounds ty x = true <-> scalar_min ty <= x <= scalar_max ty.
+  scalar_in_bounds ty x = true ↔ scalar_min ty <= x <= scalar_max ty.
 Proof.
 split. now apply scalar_in_bounds_valid.
 intro H.
@@ -257,16 +261,16 @@ cut (to_Z (bounded_scalar_succ n b) - to_Z 1 %usize = to_Z n).
 - apply Z.pred_succ.
 Qed.
 
-Lemma mk_scalar_success (ty: scalar_ty) {n: Z} : (scalar_min ty <= n) -> (n <= scalar_max ty) -> ∃x, mk_scalar ty n = Return x.
+Lemma mk_scalar_success (ty: scalar_ty) {n: Z} : (scalar_min ty <= n) → (n <= scalar_max ty) → ∃x, mk_scalar ty n = Return x.
 Proof.
 intros Hmin Hmax.
 exists (mk_bounded_scalar ty n Hmin Hmax).
 apply mk_bounded_scalar_success.
 Qed.
 
-Lemma usize_peano_ind (P: usize -> Prop) :
-  P (0%usize) ->
-  (∀n, ∀b: to_Z n < usize_max, P n -> P (bounded_scalar_succ n b)) ->
+Lemma usize_peano_ind (P: usize → Prop) :
+  P (0%usize) →
+  (∀n, ∀b: to_Z n < usize_max, P n → P (bounded_scalar_succ n b)) →
   ∀n, P n.
 Proof.
 intros base rec n.
@@ -280,19 +284,19 @@ destruct x.
   set (y := 0%usize).
   assert (H : x = y) by now apply usize_nat_inj.
   now apply (eq_ind y P base x).
-- (* nat_ind: P P0 (f:∀n.Pn->PSn) -> ∀n.Pn *)
+- (* nat_ind: P P0 (f:∀n.Pn→PSn) → ∀n.Pn *)
   admit.
 Admitted.
 
 (* Not trivial to generalize due to eq_refl in %usize. The zero and successor case are done to ease recursion *)
-Lemma usize_nat_zero {n: usize} : (usize_to_nat n = 0%nat) <-> (n = 0 %usize).
+Lemma usize_nat_zero {n: usize} : (usize_to_nat n = 0%nat) ↔ (n = 0 %usize).
 Proof.
 split ; intro H.
 - now apply usize_nat_inj, H.
 - now rewrite H.
 Qed.
 
-Lemma usize_nat_succ {n: usize} {m: nat} : (usize_to_nat n = S m) -> (∃i, usize_sub n 1 %usize = Return i).
+Lemma usize_nat_succ {n: usize} {m: nat} : (usize_to_nat n = S m) → (∃i, usize_sub n 1 %usize = Return i).
 Proof.
 destruct n. intro I.
 destruct x.
@@ -306,7 +310,7 @@ assert (Hmax: z - 1 <= scalar_max Usize) by lia.
 apply (mk_scalar_success Usize Hmin Hmax).
 Qed.
 
-Lemma usize_to_nonzero {n: usize} : n <> 0%usize <-> ∃m, usize_to_nat n = S m.
+Lemma usize_to_nonzero {n: usize} : n <> 0%usize ↔ ∃m, usize_to_nat n = S m.
 Proof.
 split.
 - intros H.
@@ -325,7 +329,7 @@ Qed.
 
 (* There are may similar lemmas to be defined *)
 Lemma scalar_eqb_eq {ty} {n m: scalar ty} :
-    (n s= m) = true <-> n = m.
+    (n s= m) = true ↔ n = m.
 Proof.
 unfold scalar_eqb.
 split ; intro.
@@ -334,14 +338,14 @@ split ; intro.
 Qed.
 
 Lemma scalar_eqb_ne {ty} {n m: scalar ty} :
-(n s= m) = false <-> n <> m.
+(n s= m) = false ↔ n <> m.
 Proof.
 rewrite <-(not_true_iff_false (n s= m)).
 apply (neg_equiv scalar_eqb_eq).
 Qed.
 
 Lemma Z_eqb_ne {n m: Z} :
-(n =? m) = false <-> n <> m.
+(n =? m) = false ↔ n <> m.
 Proof.
 rewrite <-(not_true_iff_false (n =? m)).
 apply (neg_equiv (Z.eqb_eq _ _)).
@@ -368,7 +372,7 @@ Ltac ltac_new_id2 prefix id suffix :=
   let new := constr:((prefix ++ old ++ suffix)%string) in
   string_to_ident new.
 
-(* Written as a tactic to exploit proof by rewriting - I may miss another way *)
+(* Written as a tactic to exploit proof by rewriting - I may miss another way: very hacky and fragile *)
 Ltac scalar_success_tac X B :=
   let H := fresh in
   unfold mk_scalar;
@@ -390,17 +394,23 @@ Proof.
 exact (proj2_sig n).
 Qed.
 
+Lemma V_vec_bounds {T} (v: vec T) :
+  usize_min <= vec_length v <= usize_max.
+Proof.
+exact (vec_len_in_usize v).
+Qed.
+
 Lemma S_scalar_Z_inj {ty} (n m: scalar ty) :
-  to_Z n = to_Z m -> n = m.
+  to_Z n = to_Z m → n = m.
 Proof.
 destruct m, n.
 apply ProofIrrelevanceTheory.subset_eq_compat.
 Qed.
 
 Lemma S_mk_bounded ty (x: Z) :
-  scalar_min ty <= x <= scalar_max ty ->
+  scalar_min ty <= x <= scalar_max ty →
   ∃n, mk_scalar ty x = Return n
-   /\ to_Z n = x.
+   ∧ to_Z n = x.
 Proof.
 intro B.
 pose (n := (exist _ x B): scalar ty).
@@ -410,9 +420,9 @@ scalar_success_tac x B.
 Qed.
 
 Lemma S_add_bounded {ty} (n m: scalar ty) :
-  scalar_min ty <= (to_Z n) + (to_Z m) <= scalar_max ty ->
+  scalar_min ty <= (to_Z n) + (to_Z m) <= scalar_max ty →
   ∃x, scalar_add n m = Return x
-   /\ to_Z x = (to_Z n) + (to_Z m).
+   ∧ to_Z x = (to_Z n) + (to_Z m).
 Proof.
 intro B.
 pose (x := (exist _ (to_Z n + to_Z m) B): scalar ty).
@@ -422,10 +432,23 @@ unfold scalar_add.
 scalar_success_tac (to_Z n + to_Z m) B.
 Qed.
 
+(* Alternative shape for the lemma above. *)
+Lemma S_add_bounded2 {T} (n m: scalar T) :
+  scalar_min T <= (to_Z n) + (to_Z m) <= scalar_max T →
+  match scalar_add n m with
+  | Return x => to_Z x = (to_Z n) + (to_Z m)
+  | Fail_ _ => False
+  end.
+Proof.
+intro H.
+destruct (S_add_bounded n m H) as (x, (eq, P)).
+now rewrite eq.
+Qed.
+
 Lemma S_sub_bounded {ty} (n m: scalar ty) :
-  scalar_min ty <= (to_Z n) - (to_Z m) <= scalar_max ty ->
+  scalar_min ty <= (to_Z n) - (to_Z m) <= scalar_max ty →
   ∃x, scalar_sub n m = Return x
-   /\ to_Z x = (to_Z n) - (to_Z m).
+   ∧ to_Z x = (to_Z n) - (to_Z m).
 Proof.
 (* TODO: Factorize common stuff more *)
 intro B.
@@ -437,9 +460,9 @@ scalar_success_tac (to_Z n - to_Z m) B.
 Qed.
 
 Lemma S_mul_bounded {ty} (n m: scalar ty) :
-  scalar_min ty <= (to_Z n) * (to_Z m) <= scalar_max ty ->
+  scalar_min ty <= (to_Z n) * (to_Z m) <= scalar_max ty →
   ∃x, scalar_mul n m = Return x
-   /\ to_Z x = (to_Z n) * (to_Z m).
+   ∧ to_Z x = (to_Z n) * (to_Z m).
 Proof.
 intro B.
 pose (x := (exist _ (to_Z n * to_Z m) B): scalar ty).
@@ -450,25 +473,25 @@ scalar_success_tac (to_Z n * to_Z m) B.
 Qed.
 
 Lemma S_div_bounded {ty} (n m: scalar ty) :
-  to_Z m <> 0 ->
-  scalar_min ty <= (to_Z n) / (to_Z m) <= scalar_max ty ->
+  to_Z m <> 0 ∧ scalar_min ty <= (to_Z n) / (to_Z m) <= scalar_max ty →
   ∃x, scalar_div n m = Return x
-   /\ to_Z x = (to_Z n) / (to_Z m).
+   ∧ to_Z x = (to_Z n) / (to_Z m).
 Proof.
-intros B0 B.
-pose (x := (exist _ (to_Z n / to_Z m) B): scalar ty).
+intro B.
+destruct B as (B0, B1).
+pose (x := (exist _ (to_Z n / to_Z m) B1): scalar ty).
 exists x.
 split. 2: reflexivity.
 unfold scalar_div.
 remember (to_Z m =? 0) as b.
 destruct b. 1: intuition.
-scalar_success_tac (to_Z n / to_Z m) B.
+scalar_success_tac (to_Z n / to_Z m) B1.
 Qed.
 
 Lemma S_rem_bounded {ty} (n m: scalar ty) :
-  scalar_min ty <= Z.rem (to_Z n) (to_Z m) <= scalar_max ty ->
+  scalar_min ty <= Z.rem (to_Z n) (to_Z m) <= scalar_max ty →
   ∃x, scalar_rem n m = Return x
-   /\ to_Z x = Z.rem (to_Z n) (to_Z m).
+   ∧ to_Z x = Z.rem (to_Z n) (to_Z m).
 Proof.
 intro B.
 pose (x := (exist _ (Z.rem (to_Z n) (to_Z m)) B): scalar ty).
@@ -478,24 +501,25 @@ unfold scalar_rem.
 scalar_success_tac (Z.rem (to_Z n) (to_Z m)) B.
 Qed.
 
+(* TODO: Complete proofs. *)
 Lemma V_push_back_bounded {T} (v: vec T) (x: T) :
-  vec_length v < usize_max ->
+  vec_length v < usize_max →
   ∃w, vec_push_back T v x = Return w
-   /\ vec_to_list w = (vec_to_list v) ++ [x].
+   ∧ vec_to_list w = (vec_to_list v) ++ [x].
 Proof.
 Admitted.
 
 Lemma V_index_mut_fwd_bounded {T} (v: vec T) (i: usize) :
-  to_Z i < vec_length v ->
+  to_Z i < vec_length v →
   ∃x, vec_index_mut_fwd T v i = Return x
-   /\ nth_error (vec_to_list v) (usize_to_nat i) = Some x.
+   ∧ nth_error (vec_to_list v) (usize_to_nat i) = Some x.
 Proof.
 Admitted.
 
 Lemma V_index_mut_back_bounded {T} (v: vec T) (i: usize) (x: T) :
-  to_Z i < vec_length v ->
+  to_Z i < vec_length v →
   ∃w, vec_index_mut_back T v i x = Return w
-   /\ vec_to_list w = replace_list (vec_to_list v) (usize_to_nat i) x.
+   ∧ vec_to_list w = replace_list (vec_to_list v) (usize_to_nat i) x.
 Proof.
 Admitted.
 
@@ -505,6 +529,42 @@ unfold usize_to_nat.
 apply Z2Nat.id.
 apply (S_scalar_bounds n).
 Qed.
+
+(* Issues with trying to fit destruct_eqb in a monadic lemma :
+- No premisses.
+- Not triggered on a result type.
+- No equation of the shape "∃x. ... = Return x".
+- No postcondition rewrite rule.
+At best, it only provides an "apply".
+
+Where should it fit ?
+- Separate the function accessing the 'head variable'.
+- Add a typeclass to apply on 'head variable' more generally than the whole goal.
+
+New roles for high-level tactics ?
+- "oaSimpl" something applied recursively which simplifies & uniformises the context (including the goal).
+- "oaStep" something applied once on the 'head variable' to progress on the goal.
+
+It means that "oaStep" must be complexified to accomodate the 'match' shape.
+*)
+Lemma S_eqb_dec {ty} (n m: scalar ty) :
+  True →
+  ∃x, scalar_eqb n m = x
+   ∧ (x = true ∧ n = m) ∨ (x = false ∧ n ≠ m).
+Proof.
+Admitted.
+
+(* An apply + rewrite of the lemma above gives us grosso modo that, which is very close to "Z.eqb_dec" :
+
+We want non-monadic lemmas which apply to the HV in "aeStep", and perhaps corresponding simplifying lemmas in "aeSimpl" :
+- "aeStep" intro "Z.eqb_dec" ("bounded hyp" TC ?).
+- "aeSimpl" destruct equations on booleans :
+  + "?A = true ↔ ?B" ~> destruct A, get true ⊢ B and false ⊢ ¬B.
+*)
+Lemma S_eqb_dec2 {ty} (n m: scalar ty) :
+  (n s= m) = true ↔ n = m.
+Proof.
+Admitted.
 
 (*  +-------------------+
     | Tactics - helpers |
@@ -529,9 +589,17 @@ Ltac intro_scalar_bounds n :=
   assert (H := S_scalar_bounds n);
   simpl in H.
 
+(* Registers the bounds of the given vector in a new hypothesis. *)
+Ltac intro_vec_bounds v :=
+  let H_id := ltac_new_id ""%string v "_bounds"%string in
+  let H := fresh H_id in
+  assert (H := V_vec_bounds v);
+  simpl in H.
+
 (* Does not create an identifier based on n.
    Used for unknown scalar parameters which could be expressions.
    TODO: Match identifiers VS expressions to know which tactic to call.
+   TODO: Search if the bounds is already in the hypothesis.
 *)
 Ltac intro_scalar_anon_bounds n :=
   let H := fresh in
@@ -1017,7 +1085,7 @@ Ltac siphon fuel :=
     fold f
   ) in
   (* Not lazy to allow failing on some match *)
-  match goal with
+  lazymatch goal with
   (* TODO: How to match the already unfolded fixpoint ?
   | [ |- context[ (fix _ (match _ with _ => _ end)) fuel ] ] =>
     destruct fuel;
@@ -1051,17 +1119,518 @@ Ltac siphon fuel :=
   It's not clear however if it can really be useful.
 *)
 
-Ltac make_progress :=
-  lazymatch goal with
-  | [ |- context[ to_Z ?A =? to_Z ?B ] ] => destruct_eqb A B
-  | [ |- context[ scalar_add ?A ?B ] ] => rewrite_scalar_add A B
-  | [ |- context[ scalar_sub ?A ?B ] ] => rewrite_scalar_sub A B
-  | [ |- context[ scalar_mul ?A ?B ] ] => rewrite_scalar_mul A B
-  | [ |- context[ scalar_div ?A ?B ] ] => rewrite_scalar_div A B
-  | [ |- context[ vec_push_back _ ?A ?B ] ] => rewrite_vec_push_back A B
+(* Introduce a term, with its bounds if it's a scalar. *)
+Ltac aeIntro n :=
+  intro n;
+  match type of n with
+  | scalar _ => intro_scalar_bounds n
+  | vec _ => intro_vec_bounds n
+  | _ => idtac
   end.
-(* (λx.if x then y else z)a *)
 
+(* Simplify scalar & vec expressions.
+   TODO: must fail when not applied.
+   TODO: Vectors of known elements to lists.
+   TODO: Targeted simplifications can be avoided if simpl of sacalars & vec is blocked.
+   TODO: Make rewrite rules extandable by obtaining them from a typeclass or an autorewrite hint database (for e.g. "usize_nat_to_Z").
+*)
+Ltac aeSimpl :=
+  repeat
+ (rewrite usize_nat_to_Z in * ||
+  rewrite res_bind_value in * ||
+  rewrite res_bind_id in * ||
+  lazymatch goal with
+  (* Scalar constants *)
+  | |- context[ to_Z (eval_result_refl ?A eq_refl) ] =>
+      simpl (to_Z (eval_result_refl A eq_refl))
+  | H: context[ to_Z (eval_result_refl ?A eq_refl) ] |- _ =>
+      simpl (to_Z (eval_result_refl A eq_refl)) in H
+  end).
+
+(* Pick and apply a custom tactic to the given expression. *)
+(* TODO: other operations (scalar_neg/cast/leb/..., vec_push/insert/index/...) *)
+Ltac aeStepLeaf P n :=
+  lazymatch P with
+  | to_Z ?A =? to_Z ?B => destruct_eqb A B as n
+  | scalar_add ?A ?B => rewrite_scalar_add A B as n
+  | scalar_sub ?A ?B => rewrite_scalar_sub A B as n
+  | scalar_mul ?A ?B => rewrite_scalar_mul A B as n
+  | scalar_div ?A ?B => rewrite_scalar_div A B as n
+  | scalar_rem ?A ?B => rewrite_scalar_rem A B as n
+  | vec_push_back _ ?A ?B => rewrite_vec_push_back A B as n
+  | vec_index_mut_fwd _ ?A ?B => rewrite_vec_index_mut_fwd A B as n
+  | vec_index_mut_back _ ?A ?B ?C => rewrite_vec_index_mut_back A B C as n
+  
+  | _ => fail "no Aeneas lemma could be automatically applied"
+  end.
+
+(* TODO: Should we go under function arguments and if/match branches ?
+*)
+Ltac aeStepRec G n :=
+  lazymatch G with
+  (* Go under implications *)
+  | forall _, _ => aeIntro n
+  | _ → _ => aeIntro n
+  (* TODO Desugarized match - Go under blocking eliminations *)
+  | if ?A then _ else _ => aeStepRec A n
+  | match ?A with _ => _ end => aeStepRec A n
+  (* Go under the error monad *)
+  | Primitives.bind ?A _ => aeStepRec A n
+  (* Go under equation *)
+  | ?A = ?B => aeStepRec A n || aeStepRec B n
+  (* Try to apply a lemma *)
+  | ?P => aeStepLeaf P n
+  end.
+
+Ltac aeStepGoal n :=
+  lazymatch goal with
+  (* Apply injective lemmas on scalar & vec equations *)
+  | |- ?A = ?B =>
+      match type of A with
+      | scalar _ => apply scalar_Z_inj
+      | vec _ => apply vec_list_inj
+      | _ => aeStepRec A n || aeStepRec B n
+      end
+  (* Proceed normally *)
+  | |- ?G => aeStepRec G n
+  end;
+  aeSimpl.
+
+(* TODO: Find how to match an hypothesis by its name. *)
+Ltac aeStepHyp h n :=
+  lazymatch type of h with
+  | ?H => aeStepRec H n
+  end;
+  aeSimpl.
+
+(* TODO: Authorize "aeStep in *" by iterating on all hypothesis.
+It does not seems trivial (at least 12y ago):
+https://coq-club.inria.narkive.com/84wy4cCg/ltac-iteration-on-all-hypothesis#post4
+*)
+
+Tactic Notation "aeStep" :=
+  let n := fresh in
+  aeStepGoal n.
+
+Tactic Notation "aeStep" "as" simple_intropattern(n) :=
+  aeStepGoal n.
+
+Tactic Notation "aeStep" "in" simple_intropattern(h) :=
+  let n := fresh in
+  aeStepHyp h n.
+
+Tactic Notation "aeStep" "as" simple_intropattern(n) "in" simple_intropattern(h) :=
+  aeStepHyp h n.
+
+Tactic Notation "aeStep" "in" simple_intropattern(h) "as" simple_intropattern(n) :=
+  aeStepHyp h n.
+
+(*  +--------------+
+    | Open version |
+    +--------------+
+*)
+(*
+The goal here is to develop a modularized tactic to progress on a given goal by simplifying & solving elements which may be given by the user.
+To do that, a high-level "aeProgress" tactic will be built from 3 components:
+- "aeStep" which inspects the goal head variable and lookup a lemma to apply to it.
+- "aeSimpl" which uniformises the hypotheses by simplifying it and looking up bounds to introduce.
+- "aeSolve" which aims to resolve the obtained goals.
+
+For now, the prefix is changed to "oa" to avoid conflicts.
+
+TODO:
+- How to add various simplification rules/tactics to aeStep, and is it wanted ? (typically destruct_eqb, scalar_Z_inj).
+- Is the typeclass approach still good if they proliferate ?
+- 
+*)
+
+(*
+Registers lemmas that are applied by the "oaStep" tactic.
+
+The interface for monadic lemmas accept proofs of propositions of the following shape:
+"T → T₁ → ... → Tₙ → ∀x₁:T₁...∀xₙ:Tₙ, Preconditions → ∃x:T, f x₁...xₙ = Return x ∧ Postconditions"
+
+To avoid the issue with variadic arguments, we match the function applied to all of its arguments (minus the precondition).
+
+The "polymorphic" qualifier is only needed for "T → Prop", which lives one universe above.
+*)
+Polymorphic Class MonadicLemma {T} (f: result T) := {
+  monl_pre : Prop;
+  monl_post : T → Prop;
+  monl_lemma : monl_pre → ∃(x: T), f = Return x ∧ monl_post x;
+}.
+
+(* Non-monadic variant of "MonadicLemma". More versatile but less powerful : it only adds a lemma in hypothesis, assert its precondition then "destruct" the HV ("MonadicLemma" morally performs a "destruct" as well).
+TODO: Rename "MonadicLemma" ⇝ "StepMonadicLemma", "ApplicableLemma" ⇝ "StepLemma" ? To make it clear that those are used by "oaStep" & that there are similar (modulo monadicity).
+*)
+Polymorphic Class ApplicableLemma {T} (e: T) := {
+  appl_pre : Prop;
+  appl_lemma : appl_pre → Prop;
+}.
+
+(* Instances for primitives. *)
+
+Global Instance monadic_lemma_scalar_add T n m : MonadicLemma (@scalar_add T n m) :=
+  {| monl_lemma := S_add_bounded n m; |}.
+
+Global Instance monadic_lemma_scalar_mul T n m : MonadicLemma (@scalar_mul T n m) :=
+  {| monl_lemma := S_mul_bounded n m; |}.
+
+Global Instance monadic_lemma_scalar_sub T n m : MonadicLemma (@scalar_sub T n m) :=
+  {| monl_lemma := S_sub_bounded n m; |}.
+
+Global Instance monadic_lemma_scalar_div T n m : MonadicLemma (@scalar_div T n m) :=
+  {| monl_lemma := S_div_bounded n m; |}.
+
+Global Instance monadic_lemma_scalar_rem T n m : MonadicLemma (@scalar_rem T n m) :=
+  {| monl_lemma := S_rem_bounded n m; |}.
+
+Global Instance monadic_lemma_vec_push_back T v x : MonadicLemma (vec_push_back T v x) :=
+  {| monl_lemma := V_push_back_bounded v x; |}.
+
+Global Instance monadic_lemma_vec_index_mut_fwd T v i : MonadicLemma (vec_index_mut_fwd T v i) :=
+  {| monl_lemma := V_index_mut_fwd_bounded v i; |}.
+
+Global Instance monadic_lemma_vec_index_mut_back T v i x : MonadicLemma (vec_index_mut_back T v i x) :=
+  {| monl_lemma := V_index_mut_back_bounded v i x; |}.
+
+(*
+Registers types which, when instantiated by hypothesis, should expose an additional hypothesis on them (typically, to project scalars and vectors to Z and lists respectfully).
+*)
+Polymorphic Class BoundedHypothesis T := {
+  bo_hyp_prop : T → Prop;
+  bo_hyp_lemma (x: T) : bo_hyp_prop x;
+}.
+
+(* Instances for primitives.
+
+TODO: We may want to lift it in sum & product types (Bounded A & Bounded B => Bounded (A, B), ...).
+*)
+
+Global Instance bounded_hypothesis_scalar T : BoundedHypothesis (scalar T) :=
+  {| bo_hyp_lemma := S_scalar_bounds; |}.
+
+Global Instance bounded_hypothesis_vector T : BoundedHypothesis (vec T) :=
+  {| bo_hyp_lemma := V_vec_bounds; |}.
+
+(*
+Registers types to simplify equation goals on their terms with the given injective function (typically, to project scalars on Z and vectors on lists).
+
+TODO: It's not clear that it's really needed ... It helps to fully automatize scalar/vector-specific part but that's it.
+Perhaps it should be added in "oaStep" with generic lemmas to 'apply'.
+Also, same as above, we can lift it for sum & product types.
+*)
+Polymorphic Class InjectiveProjection T := {
+  injp_type : Type;
+  injp_fun : T → injp_type;
+  injp_lemma (a b: T) : injp_fun a = injp_fun b → a = b;
+}.
+
+(* Instances for primitives. *)
+
+Global Instance injective_projection_scalar T : InjectiveProjection (scalar T) :=
+  {| injp_lemma := S_scalar_Z_inj; |}.
+
+Global Instance injective_projection_vector T : InjectiveProjection (vec T) :=
+  {| injp_lemma := @vec_list_inj _; |}.
+
+(* Low-level tactic to only resolve typeclasses, without backtracking. It is strictly less powerful than e.g. "exact _". *)
+Ltac tc_solve :=
+  solve [once (typeclasses eauto)].
+
+(* TODO: Test it. The name is a bit long ... *)
+Notation monadic_oof_shape x P := match x with
+  | Return v => P v
+  | Fail_ OutOfFuel => True
+  | Fail_ Failure => False
+  end.
+
+(* Allow to swap between two formulations of statements about results:
+- The match shape, a convenient formulation for partial correctness.
+- The existential formula of monadic lemmas, which can be used by "aoStepGoal".
+*)
+Lemma monadic_shape_to_instance {T} {x: result T} {P: T → Prop} :
+  (match x with
+  | Return a => P a
+  | Fail_ OutOfFuel => True
+  | Fail_ Failure   => False
+  end)
+  ↔
+  (x ≠ Fail_ OutOfFuel →
+  ∃ a, x = Return a ∧ P a).
+Proof.
+split; destruct x; intros.
+- now exists t.
+- now destruct e.
+- assert (Return t ≠ Fail_ OutOfFuel) by easy.
+  destruct (H H0) as (x, (A, B)).
+  injection A.
+  intro C. now rewrite C.
+- destruct e. 2: trivial.
+  assert (@Fail_ T Failure ≠ Fail_ OutOfFuel) by easy.
+  now destruct (H H0).
+Qed.
+
+Lemma monadic_shape_to_instance_hyp {T} {x: result T} {P: Prop} {Q: T → Prop} :
+  (P → match x with
+  | Return a => Q a
+  | Fail_ OutOfFuel => True
+  | Fail_ Failure   => False
+  end)
+  ↔
+  (P ∧ x ≠ Fail_ OutOfFuel →
+  ∃ a, x = Return a ∧ Q a).
+Proof.
+split; intros.
+- destruct H0. assert (p := H H0).
+  now apply monadic_shape_to_instance.
+- apply monadic_shape_to_instance. intro.
+  now apply H.
+Qed.
+
+(* Can be used for automatic proof search. *)
+Lemma weaken_oof_guard {A B} {f: result A} {g: A → result B} :
+  (v ← f; g v) ≠ Fail_ OutOfFuel →
+  f ≠ Fail_ OutOfFuel.
+Proof.
+destruct f. 1: easy.
+now destruct e.
+Qed.
+
+Lemma monadic_oof_hyp {A} {f: result A} {P: A → Prop} :
+  (f ≠ Fail_ OutOfFuel →
+  match f with
+  | Return x => P x
+  | Fail_ OutOfFuel => True
+  | Fail_ Failure   => False
+  end) →
+  match f with
+  | Return x => P x
+  | Fail_ OutOfFuel => True
+  | Fail_ Failure   => False
+  end.
+Proof.
+rewrite monadic_shape_to_instance_hyp. intro H.
+assert (f ≠ Fail_ OutOfFuel) by intuition.
+revert H.
+rewrite <-monadic_shape_to_instance_hyp.
+intro.
+now apply H.
+Qed.
+
+(* Add bounds to all hypotheses that could have it. The function flow is a bit missed up due to various limitations. *)
+Ltac oaAddBounds :=
+  lazymatch goal with
+  | H: ?A |- _ =>
+    (* Continue when failing (see below) - e.g. no TC found.
+    TODO: Find a cleaner mechanism.
+    *)
+    let TC := fresh "TC" in
+    tryif pose (TC := (ltac:(tc_solve): BoundedHypothesis A))
+    then (
+      (* Create bounds. Done before checking that it already exists because we need its simplified type to do the match. *)
+      let bounds := ltac_new_id ""%string H "_bounds"%string in
+      assert (bounds := bo_hyp_lemma H);
+      simpl in bounds;
+      (* Push it on the goal. *)
+      clear TC;
+      let T := type of bounds in
+      revert bounds;
+      lazymatch goal with
+      | B: T |- _ =>
+        (* Bounds already exists : keep it, remove the new one to keep the previous name. *)
+        intro;
+        clear bounds;
+        revert B;
+        (* Continue. *)
+        revert H;
+        oaAddBounds;
+        intro;
+        pose (YES := 1)
+      | _ =>
+        (* Continue, then reintroduce the new bounds. *)
+        revert H;
+        oaAddBounds;
+        intro;
+        intro
+      end
+    )
+    else (
+      (* No "BoundedHypothesis" typeclass : continue. *)
+      revert H;
+      oaAddBounds;
+      intro
+    )
+  (* No more hypothesis. *)
+  | _ => idtac
+  end.
+
+(* Simplify the goal with "InjectiveProjection". *)
+Ltac oaInjectEqGoal :=
+  lazymatch goal with
+  | |- @eq ?A ?x ?y =>
+    let TC := fresh "TC" in
+    let f := fresh "f" in
+    pose (TC := (ltac:(tc_solve): InjectiveProjection A));
+    pose (f := injp_lemma x y);
+    simpl in f;
+    apply f;
+    clear f;
+    clear TC
+  end.
+
+(* Uniformize the context and goal with various simplifications. TODO: put equalities in an "autorewrite" hint database. *)
+Ltac oaSimpl :=
+  oaAddBounds;
+  try oaInjectEqGoal;
+  try repeat (rewrite usize_nat_to_Z in *);
+  try repeat (rewrite res_bind_value in *);
+  try repeat (rewrite res_bind_id in *);
+  repeat lazymatch goal with
+  (* Scalar constants *)
+  | |- context[ to_Z (eval_result_refl ?A eq_refl) ] =>
+      simpl (to_Z (eval_result_refl A eq_refl))
+  | H: context[ to_Z (eval_result_refl ?A eq_refl) ] |- _ =>
+      simpl (to_Z (eval_result_refl A eq_refl)) in H
+  end.
+  
+(* Solves the given goal with "lia" and other tactics or fails. *)
+Ltac oaSolveGoal :=
+  oaSimpl;
+  easy || lia ||
+  lazymatch goal with
+  | |- _ ∧ _ => split; oaSolveGoal
+  | _ => fail "couldn't solve the goal"
+  end.
+
+(* Applies an hypothesis about the fuel to the goal if needed, of the shape "... ≠ Fail_ OutOfFuel". *)
+Ltac oaApplyOofHyp H_oof :=
+  let rec_on_wedge H_oof := (
+    split;
+    lazymatch goal with
+    | |- _ ≠ Fail_ OutOfFuel => oaApplyOofHyp H_oof
+    | |- _ => idtac
+    end
+  ) in
+  lazymatch goal with
+  (* It's a left or right condition. *)
+  | |- _ ∧ _ ≠ Fail_ OutOfFuel => rec_on_wedge H_oof
+  | |- _ ≠ Fail_ OutOfFuel ∧ _ => rec_on_wedge H_oof
+  (* The goal may be weaker than the hypothesis. *)
+  | |- _ ≠ Fail_ OutOfFuel =>
+    apply H_oof ||
+    apply (weaken_oof_guard H_oof)
+  | |- _ => idtac
+  end.
+
+(* TODO: "simpl"s in pre/L should only unfold the typeclass fields. *)
+Ltac oaApplyMonadicLemma f res H_oof :=
+  (* Lookup the monadic lemma via its typeclass *)
+  let TC := fresh "TC" in
+  pose (TC := (ltac:(tc_solve): MonadicLemma f));
+  simpl in TC;
+
+  (* Add a goal for preconditions *)
+  let pre := fresh "pre" in
+  assert (pre: monl_pre);
+  lazymatch goal with
+  | |- monl_pre =>
+    simpl;
+    oaApplyOofHyp H_oof;
+    try oaSolveGoal
+  | _ =>
+    simpl in pre;
+  
+    (* Instantiate the lemma with its preconditions. *)
+    let L := fresh "L" in
+    assert (L := monl_lemma pre);
+    simpl in L;
+
+    (* Split it into the new variable, the equation and the postconditions. *)
+    let H := fresh in
+    destruct L as (res, H);
+    let eq := fresh "eq" in
+    let post := ltac_new_id "H"%string res ""%string in
+    destruct H as (eq, post);
+
+    (* Rewrite the function application then clear up the context.
+    TODO: Add "try rewrite res_bind_value/id" for the rewritten HV.
+    *)
+    rewrite eq;
+    clear eq;
+    clear pre
+  end;
+  clear TC.
+
+Ltac oaApplyNonMonadicLemma f res :=
+  let TC := fresh "TC" in
+  pose (TC := (ltac:(tc_solve): ApplicableLemma f));
+  simpl in TC;
+  
+  (* Add a goal for preconditions. *)
+  let pre := fresh "pre" in
+  assert (pre: appl_pre);
+  lazymatch goal with
+  | |- appl_pre =>
+    simpl;
+    oaApplyOofHyp H_oof;
+    try oaSolveGoal
+  | ?A =>
+    simpl in pre;
+    
+    (* Instantiate the lemma then destruct the HV. *)
+    assert (res := appl_lemma pre);
+    simpl in res;
+    clear pre;
+    destruct A
+  end;
+  clear TC.
+
+(* Recursively reaches the head variable. *)
+Ltac oaStepRec G n H_oof :=
+  lazymatch G with
+  (* Go under implications.
+  TODO: We may want to fail because rewriting under abstractions won't work anyway.
+  *)
+  | ∀ _, ?A => oaStepRec A n H_oof
+  | _ → ?A => oaStepRec A n H_oof
+  (* Go under blocking elimination. *)
+  | match ?A with _ => _ end => oaStepRec A n H_oof
+  (* Go under the error monad. *)
+  | Primitives.bind ?A _ => oaStepRec A n H_oof
+  (* Go under the equation left side. *)
+  | ?A = ?B => oaStepRec A n H_oof
+  (* Try to apply a monadic lemma. *)
+  | ?P => oaApplyMonadicLemma P n H_oof
+  end.
+
+(* Executes "t1" then "t2", even if "t1" fails (in which case an error is send).
+TODO: How to re-throw an error instead of creating a new one ? We don't want to loose e.g. its error message.
+*)
+Tactic Notation "try_" tactic(t1) "finally" tactic(t2) :=
+  tryif (t1)
+  then  (t2)
+  else ((t2); fail).
+
+Ltac oaStep n :=
+  (* Add a temporary hypothesis on oof for partial monadic goals. *)
+  lazymatch goal with
+  | |- match ?X with
+      | Return v => _
+      | Fail_ f => match f with
+        | OutOfFuel => True
+        | Failure => False
+      end end =>
+    let H_oof := fresh "oof_hyp" in
+    apply monadic_oof_hyp;
+    intro H_oof;
+    try_ (oaStepRec X n H_oof)
+    finally (clear H_oof)
+
+  | |- ?G => 
+    let H_oof := fresh "no_oof_hypothesis" in
+    oaStepRec G n H_oof
+  end.
 
 (*  +-------+
     | Tests |
@@ -1073,53 +1642,134 @@ Fixpoint usize_identity (fuel: nat) (s: usize) : result usize :=
   | 0%nat => Fail_ OutOfFuel
   | S fuel =>
     if (s s= 0%usize) then Return 0%usize else
-      x <- usize_sub s (1%usize);
-      y <- usize_identity fuel x;
+      x ← usize_sub s (1%usize);
+      y ← usize_identity fuel x;
       usize_add y (1%usize)
   end.
 
 Lemma usize_identity_shape fuel s :
+  True ->
   match usize_identity fuel s with
   | Return v => s = v
   | Fail_ OutOfFuel => True
   | Fail_ Failure   => False
   end.
 Proof.
+intro TT.
 (* induction *)
 revert fuel.
 induction_usize_to_nat s as S;
 intro fuel;
 siphon fuel;
-destruct_eqb s (0%usize) as Seq0.
+destruct_eqb as Seq0.
 
 (* 0 case *)
-1: now apply scalar_Z_inj.
+1: now oaSolveGoal.
 
 (* successor case: *)
-
-intro_scalar_bounds s.
-rewrite_scalar_sub s (1%usize) as r.
-simpl (to_Z 1 %usize) in *.
+oaSimpl.
+oaStep r.
+simpl.
 
 (* Apply IH *)
 assert (B: usize_to_nat r = S). 1: {
   (* I'm sure there is a simple tactic for that ... *)
   cut (Z.of_nat (usize_to_nat r) = Z.of_nat S).
-  intuition.
-  (* Can this fit in the induction ? *)
-  rewrite usize_nat_to_Z.
-  lia.
+  now intuition.
+  oaSolveGoal.
 }
 assert (H := IHS r B fuel).
 
-destruct (usize_identity fuel r). 2: exact H.
-rewrite res_bind_value.
+destruct (usize_identity fuel r). 2: oaSolveGoal.
+simpl.
 rewrite <-H.
 
-rewrite_scalar_add r (1%usize) as r0.
-simpl (to_Z 1 %usize) in *.
-apply scalar_Z_inj.
-lia.
+oaStep r0.
+oaSolveGoal.
+Qed.
+
+(* Want to go both ways: shape <=> ¬oof → instance *)
+
+Global Instance monadic_lemma_usize_identity fuel s : MonadicLemma (usize_identity fuel s) :=
+  {| monl_lemma := proj1 monadic_shape_to_instance_hyp (usize_identity_shape fuel s); |}.
+
+Definition add_ids fuel s :=
+  a ← usize_identity fuel s;
+  scalar_add a a.
+
+Lemma add_ids_shape fuel s :
+  to_Z s + to_Z s <= usize_max →
+  match add_ids fuel s with
+  | Fail_ OutOfFuel => True
+  | Fail_ Failure   => False
+  | Return a => to_Z a = to_Z s + to_Z s
+  end.
+Proof.
+intro.
+oaSimpl.
+unfold add_ids.
+oaStep n.
+
+(* 
+COPY-PASTED "oaAddBounds" applied to "s".
+Why does it match the hypothesis here and not in "oaSimpl", which duplicates bounds ?
+*)
+let TC := fresh "TC" in
+tryif pose (TC := (ltac:(tc_solve): BoundedHypothesis usize))
+then (
+  (* Create bounds. Done before checking that it already exists because we need its simplified type to do the match. *)
+  let bounds := ltac_new_id ""%string s2 "_bounds"%string in
+  assert (bounds := bo_hyp_lemma s);
+  simpl in bounds;
+  (* Push it on the goal. *)
+  clear TC;
+  let T := type of bounds in
+  revert bounds;
+  lazymatch goal with
+  | B: T |- _ =>
+    (* Bounds already exists : keep it, remove the new one to keep the previous name. *)
+    intro;
+    clear bounds;
+    revert B;
+    (* Continue. *)
+    pose (YES := 1)
+  | _ =>
+    (* Continue, then reintroduce the new bounds. *)
+    pose (NO := 0)
+  end
+)
+else (
+  (* No "BoundedHypothesis" typeclass : continue. *)
+  pose (BRUH := -1)
+).
+intro.
+
+
+
+
+oaSimpl. (* TODO: Why two bounds ? *)
+rewrite <-Hn.
+now oaStep m.
+Qed.
+
+(* Same lemma as above, but without the machinery above. *)
+Lemma add_ids_shape2 fuel s :
+  to_Z s + to_Z s <= usize_max →
+  match add_ids fuel s with
+  | Fail_ OutOfFuel => True
+  | Fail_ Failure   => False
+  | Return a => to_Z a = to_Z s + to_Z s
+  end.
+Proof.
+intro.
+oaSimpl.
+unfold add_ids.
+(* "oaStep" replaces this assert + destruct + 2: trivial. *)
+assert (P := usize_identity_shape fuel s I).
+destruct (usize_identity fuel s). 2: trivial.
+simpl.
+rewrite <-P.
+now oaStep m.
 Qed.
 
 End Primitives_Ext.
